Add Constr and Case in AST, modify definitions, admit a few proofs

src/PlutusIR/Semantics/Dynamic/Substitution.v
@@ -78,6 +78,10 @@ Function subst (x : string) (s : Term) (t : Term) {struct t} : Term :=
       IWrap F T (subst x s t0)
   | Unwrap t0 =>
       Unwrap (subst x s t0)
+  | Constr i ts =>
+      Constr i (map (subst x s) ts)
+  | Case t ts =>
+      Case (subst x s t) (map (subst x s) ts)
   end
 
 with subst_b (x : string) (s : Term) (b : Binding) {struct b} : Binding :=
@@ -94,6 +98,71 @@ Notation "'[' s '/' x ']' t" := (subst x s t) (in custom plutus_term at level 20
 Notation "'[' s '/' x '][b]' b" := (subst_b x s b) (in custom plutus_term at level 20, x constr).
 Notation "'[' s '/' x '][bnr]' bs" := (@subst_bnr x s bs) (in custom plutus_term at level 20, x constr).
 Notation "'[' s '/' x '][br]' bs" := (@subst_br  x s bs) (in custom plutus_term at level 20, x constr).
+
+
+(* Unfolding lemmas *)
+(* TODO: do this with equations 1.3 instead. Using "Function" seems to brittle:
+  it used to generate subst_equation unfolding lemma, but it changed when I
+  added cases for Constr and Case, which use map.
+*)
+
+Lemma subst_unfold x s t : subst x s t =
+  match t with
+  | Let NonRec bs t0 =>
+      Let NonRec (@subst_bnr' subst_b x s bs)
+        (if existsb (eqb x) (bvbs bs)
+          then t0
+          else subst x s t0
+        )
+  | Let Rec bs t0 =>
+      if existsb (eqb x) (bvbs bs)
+        then
+          Let Rec bs t0
+        else
+          Let Rec (@subst_br' subst_b x s bs) (subst x s t0)
+  | Var y =>
+      if x =? y
+        then s
+        else Var y
+  | TyAbs bX K t0 =>
+      TyAbs bX K (subst x s t0)
+  | LamAbs bx T t0 =>
+      if x =? bx
+        then LamAbs bx T t0
+        else LamAbs bx T (subst x s t0)
+  | Apply t1 t2 =>
+      Apply (subst x s t1) (subst x s t2)
+  | Constant u =>
+      Constant u
+  | Builtin d =>
+      Builtin d
+  | TyInst t0 T =>
+      TyInst (subst x s t0) T
+  | Error T =>
+      Error T
+  | IWrap F T t0 =>
+      IWrap F T (subst x s t0)
+  | Unwrap t0 =>
+      Unwrap (subst x s t0)
+  | Constr i ts =>
+      Constr i (map (subst x s) ts)
+  | Case t ts =>
+      Case (subst x s t) (map (subst x s) ts)
+  end.
+Proof.
+  destruct t; reflexivity.
+Qed.
+
+
+Lemma subst_b_unfold x s b : subst_b x s b =
+  match b with
+  | TermBind stricty (VarDecl y T) tb =>
+      TermBind stricty (VarDecl y T) (subst x s tb)
+  | _ => b
+  end.
+Proof.
+  destruct b; reflexivity.
+Qed.
 
 (** Multi-substitutions of terms *)
 Fixpoint msubst (ss : list (string * Term)) (t : Term) : Term :=
