src/PlutusIR/Analysis/FreeVars.v
@@ -78,6 +78,8 @@ Module Term.
      | Error ty        => []
      | Constant v      => []
      | Builtin f       => []
+     | Constr i ts     => concat (map fv ts)
+     | Case t ts       => fv t ++ concat (map fv ts)
    end
 
   with fvb rec (b : Binding) : list string :=
@@ -161,6 +163,8 @@ Module Term.
      | Error τ         => Ty.ftv τ
      | Constant v      => []
      | Builtin f       => []
+     | (Constr i ts)   => concat (map ftv ts)
+     | (Case t ts)    => ftv t ++ concat (map ftv ts)
      end
 
   with ftvb rec (b : Binding) : list string :=
