src/PlutusIR/Semantics/SemanticEquivalence/Multisubstitution/Congruence.v
@@ -493,6 +493,24 @@ Lemma msubstA_Unwrap : forall ss M ,
     msubstA ss (Unwrap M) = Unwrap (msubstA ss M).
 Proof. induction ss; intros. - reflexivity. - destruct a. eauto. Qed.
 
+Lemma msubstA_Constr : forall ss n ts ,
+    msubstA ss (Constr n ts) = Constr n (map (msubstA ss) ts).
+Proof. induction ss; intros.
+  - simpl. rewrite map_id. reflexivity.
+  - destruct a. simpl. rewrite IHss. rewrite map_map. reflexivity.
+Qed.
+
+Lemma msubstA_Case : forall ss t ts,
+    msubstA ss (Case t ts) = Case (msubstA ss t) (map (msubstA ss) ts).
+Proof.
+  induction ss; intros. 
+  - simpl. rewrite map_id. reflexivity.
+  - destruct a. 
+    simpl.
+    rewrite IHss.
+    rewrite map_map.
+    reflexivity.
+Qed.
 
 Lemma msubst_Var : forall ss x,
     closed_env ss ->
@@ -546,6 +564,8 @@ Hint Rewrite
   msubstA_TyInst
   msubstA_Unwrap
   msubstA_Var
+  msubstA_Constr
+  msubstA_Case
   : msubstA_cong.
 
 Lemma not_is_error_msubstA : forall v ss, ~ is_error v -> ~ is_error (msubstA ss v).
